Simplify State.record/record'
Resolve lingering sorrys

src/ReactorModel/Execution/State.lean
@@ -29,19 +29,11 @@ def Closed (s : State) : Prop := s.progress = s.rtr.ids .rcn
 theorem Closed.progress_Nonempty [Nontrivial s] : Closed s → s.progress.Nonempty := by
   simp_all [Closed, Nontrivial.nontrivial]  
 
-/-
-noncomputable abbrev advanceTag (s : State) (g : Time.Tag) : State := 
-  { s with s := s.s.advanceTag g }
-
-instance [Nontrivial s] : Nontrivial (s.advanceTag g) where
-  nontrivial := by simp [Nontrivial.nontrivial]
--/
-
-structure allows (s : State) (rcn : ID) : Prop where
+structure Allows (s : State) (rcn : ID) : Prop where
   deps : s.rtr.dependencies rcn ⊆ s.progress
   unprocessed : rcn ∉ s.progress
 
-theorem allows_requires_acyclic_deps {s : State} : (s.allows rcn) → (rcn >[s.rtr]< rcn) := by
+theorem Allows.requires_acyclic_deps {s : State} : (s.Allows rcn) → (rcn >[s.rtr]< rcn) := by
   intro ⟨hd, hu⟩
   by_contra h
   simp [Set.subset_def, Reactor.dependencies] at hd
@@ -196,23 +188,34 @@ theorem operation_some_to_Nontrivial (h : s.operation i = some o) : Nontrivial s
   have h := operation_to_contains h |> Reactor.ids_mem_iff_contains.mpr
   sorry
 
+
+
+
+
+
+
+
+
 structure NextTag (s : State) (next : Time.Tag) : Prop where
   mem : next ∈ s.rtr.scheduledTags
   bound : s.tag < next
   least : ∀ g ∈ s.rtr.scheduledTags, (s.tag < g) → (next ≤ g)    
 
+theorem NextTag.deterministic (n₁ : NextTag s g₁) (n₂ : NextTag s g₂) : g₁ = g₂ :=
+  sorry
+
 inductive Advance : State → State → Prop 
-  | mk : (NextTag s next) → Advance s { s with tag := next }
+  | mk : (NextTag s next) → Advance s { s with tag := next, progress := ∅ }
 
-instance Advance.preserves_Nontrivial [Nontrivial s₁] : (Advance s₁ s₂) → Nontrivial s₂
-  | mk .. => sorry
+theorem Advance.progress_empty : (Advance s₁ s₂) → s₂.progress = ∅
+  | mk .. => rfl
 
-theorem Advance.progress_empty (a : Advance s₁ s₂) : s₂.progress = ∅ :=
-  sorry
+instance Advance.preserves_Nontrivial [inst : Nontrivial s₁] : (Advance s₁ s₂) → Nontrivial s₂
+  | mk .. => ⟨inst.nontrivial⟩
 
-theorem Advance.determinisic (a₁ : Advance s s₁) (a₂ : Advance s s₂) : s₁ = s₂ :=
-  sorry
-
+theorem Advance.determinisic : (Advance s s₁) → (Advance s s₂) → s₁ = s₂
+  | mk h₁, mk h₂ => by ext1 <;> simp [h₁.deterministic h₂]
+  
 theorem Advance.tag_lt : (Advance s₁ s₂) → s₁.tag < s₂.tag
   | mk h => h.bound
 
@@ -222,80 +225,18 @@ def record [DecidableEq ID] (s : State) (rcn : ID) : State :=
 theorem record_preserves_tag (s : State) (rcn : ID) : (s.record rcn).tag = s.tag := 
   rfl
 
-theorem record_comm (s : State) (rcn₁ rcn₂ : ID) : 
-    (s.record rcn₁).record rcn₂ = (s.record rcn₁).record rcn₂ := by
-  sorry
-
-theorem mem_record_progress_self (s : State) (rcn : ID) : rcn ∈ (s.record rcn).progress := by
-  sorry
-
-variable {s : State}
-
-theorem record_progress_monotonic (rcn₁ : ID) : (rcn₁ ∈ s.progress) → rcn₁ ∈ (s.record rcn₂).progress := by
-  sorry
-
-theorem mem_record_progress (h : rcn₁ ∈ (s.record rcn₂).progress) : (rcn₁ = rcn₂ ∨ rcn₁ ∈ s.progress) := by
-  sorry
-
 theorem mem_record_progress_iff (s : State) (rcn₁ rcn₂ : ID) : 
-    rcn₁ ∈ (s.record rcn₂).progress ↔ (rcn₁ = rcn₂ ∨ rcn₁ ∈ s.progress) where
-  mp := mem_record_progress
-  mpr
-    | .inl h => h ▸ s.mem_record_progress_self rcn₁
-    | .inr h => record_progress_monotonic _ h
+    rcn₁ ∈ (s.record rcn₂).progress ↔ (rcn₁ = rcn₂ ∨ rcn₁ ∈ s.progress) := by
+  simp [record]
 
-def record' [DecidableEq ID] (s : State) : List ID → State
-  | [] => s
-  | hd :: tl => (s.record hd).record' tl
+def record' [DecidableEq ID] (s : State) (rcns : List ID) : State := 
+  { s with progress := s.progress ∪ rcns.toFinset }
 
-theorem record'_cons : (s.record i).record' l = s.record' (i :: l) := rfl
-
-theorem record'_comm (s : State) (rcns : List ID) (rcn : ID) :
-    (s.record' rcns).record rcn = (s.record rcn).record' rcns := by
-  induction rcns generalizing s rcn
-  case nil => rfl
-  case cons hd tl hi => 
-    simp [record', record_comm, hi]
-    sorry
-
-theorem record'_perm_eq (h : l₁ ~ l₂) : s.record' l₁ = s.record' l₂ := by
-  induction h generalizing s
-  case nil     => rfl
-  case cons hi => simp [record', hi]
-  case swap    => simp [record', record_comm]; sorry
-  case trans   => simp_all
-
-theorem record'_progress_monotonic (l : List ID) (h : i ∈ s.progress) : 
-    i ∈ (s.record' l).progress := by
-  induction l generalizing s i
-  case nil => assumption
-  case cons hd _ hi => exact hi $ record_progress_monotonic _ h
-
-theorem record'_cons_progress_monotonic (h : i ∈ (s.record' tl).progress) : 
-    i ∈ (s.record' $ hd :: tl).progress := by
-  simp [record', ←record'_comm, record_progress_monotonic _ h]
+theorem record'_perm_eq {s : State} (h : rcns₁ ~ rcns₂) : s.record' rcns₁ = s.record' rcns₂ := by
+  simp [record', List.toFinset_eq_of_perm rcns₁ rcns₂ h]
   
-theorem mem_list_to_mem_record'_progress (h : i ∈ l) : i ∈ (s.record' l).progress := by
-  induction l
-  case nil => contradiction
-  case cons hd tl hi =>
-    cases h
-    case head   => exact record'_progress_monotonic tl $ s.mem_record_progress_self i
-    case tail h => exact record'_cons_progress_monotonic $ hi h
-
-theorem mem_record'_progress_to_mem_progress_or_mem_list (h : i ∈ (s.record' l).progress) :
-    (i ∈ s.progress ∨ i ∈ l) := by
-  induction l generalizing s i <;> simp_all [record']
-  case cons hd tl hi =>
-    cases hi h
-    case inl h => cases mem_record_progress h <;> simp [*]
-    case inr h => simp [h]
-
-theorem mem_record'_progress_iff (s : State) (l : List ID) (i : ID) :
-    i ∈ (s.record' l).progress ↔ (i ∈ s.progress ∨ i ∈ l) where
-  mp := mem_record'_progress_to_mem_progress_or_mem_list
-  mpr 
-    | .inl h => record'_progress_monotonic l h
-    | .inr h => mem_list_to_mem_record'_progress h
+theorem mem_record'_progress_iff (s : State) (rcns : List ID) (i : ID) :
+    i ∈ (s.record' rcns).progress ↔ (i ∈ s.progress ∨ i ∈ rcns) := by
+  simp [record']
 
 end Execution.State 
